theories/simulation.v
@@ -1,100 +1,262 @@
 From Paco Require Import paco.
-From stbor Require Export properties.
+From stbor Require Export properties steps_wf.
 
-(** Configuration simulation *)
+(** State simulation *)
 
-Notation SIM_CFG := (relation (cfg bor_lang))%type.
+(* Simulated memory values: ignore tags of locations *)
+Definition sim_immediate (v1 v2: immediate) :=
+  match v1, v2 with
+  | RecV _ _ _, RecV _ _ _ => v1 = v2
+  | LitV LitPoison, LitV LitPoison => True
+  | LitV (LitInt n1), LitV (LitInt n2) => n1 = n2
+  | LitV (LitLoc l1 bor1), LitV (LitLoc l2 bor2) => l1 = l2
+  | _,_ => False
+  end.
 
-Definition _sim (sim: SIM_CFG) (ρ1_src ρ1_tgt : cfg bor_lang) : Prop :=
-  (* Wf ρ1_src → Wf ρ1_tgt → *)
-  ∀ σ1_src σ1_tgt,
-  (* σ1_src, σ1_tgt are new states by other threads' interferences *)
-  Wf σ1_src → Wf σ1_tgt →
-  future_state ρ1_src.2 σ1_src → future_state ρ1_tgt.2 σ1_tgt →
-  (* σ1_src, σ1_tgt are related *)
-  sim_state σ1_src σ1_tgt →
-  (* (1) If `ρ1_tgt` is terminal, then `ρ1_src` terminates with τ steps. *)
-  (terminal ρ1_tgt.1 → ∃ Ts2_src σ2_src,
-      rtc τstep (ρ1_src.1, σ1_src) (Ts2_src, σ2_src) ∧
-      sim_state σ2_src σ1_tgt ∧ terminal Ts2_src) ∧
-  (* (2) If `ρ1_tgt` steps to `ρ2_tgt` with observation o, then exists `ρ2_src`
-         s.t. `ρ1_src` steps to `ρ2_src` with observation o AND
-         ρ2_src and ρ2_tgt related by sim. *)
-  (∀ ρ2_tgt tid_tgt ev_tgt,
-    one_step (ρ1_tgt.1, σ1_tgt) tid_tgt ev_tgt ρ2_tgt → ∃ ρ2_src tid_src ev_src,
-      one_step (ρ1_src.1, σ1_src) tid_src ev_src ρ2_src ∧
-      externally_equiv ev_src ev_tgt ∧
-      sim_state ρ1_src.2 ρ2_tgt.2 ∧ sim ρ2_src ρ2_tgt).
+Definition sim_val (v1 v2: val) :=
+  match v1, v2 with
+  | ImmV v1, ImmV v2 => sim_immediate v1 v2
+  | TValV vs1, TValV vs2 =>
+    length vs1 = length vs2 ∧
+    ∀ i v1 v2, vs1 !! i = Some v1 → vs2 !! i = Some v2 → sim_immediate v1 v2
+  | PlaceV l1 tg1 T1, PlaceV l2 tg2 T2 => l1 = l2
+  | _, _ => False
+  end.
 
-Lemma _sim_monotone : monotone2 _sim.
+Definition sim_val_expr (e1 e2: expr) :=
+  ∀ v2, to_val e2 = Some v2 → ∃ v1, to_val e1 = Some v1 ∧ sim_val v1 v2.
+
+(* Simulated state *)
+(* - cheap: Target memory is simulated by source memory
+   - cpro: Call states are the same
+   - cstk: TODO missing relation between stacks
+   - cclk: TODO missing relation between tag clocks *)
+Record sim_state (σ_src σ_tgt: state) := {
+  sim_state_mem_dom : dom (gset loc) σ_src.(cheap) ≡ dom (gset loc) σ_tgt.(cheap);
+  sim_state_stack_dom : dom (gset loc) σ_src.(cstk) ≡ dom (gset loc) σ_tgt.(cstk);
+  sim_state_protectors : σ_src.(cpro) = σ_tgt.(cpro);
+  sim_state_mem : ∀ l v2,
+    σ_tgt.(cheap) !! l = Some v2 → ∃ v1, σ_src.(cheap) !! l = Some v1 ∧ sim_immediate v1 v2;
+}.
+
+Instance sim_immediate_po : PreOrder sim_immediate.
 Proof.
-  intros ρ1_src ρ1_tgt r r' TS LE σ1_src σ1_tgt WF1 WF2 FT1 FT2 SS.
-  destruct (TS _ _ WF1 WF2 FT1 FT2 SS) as [TERM STEP]. split; [done|].
-  intros ρ2_tgt tid ev_tgt ONE.
-  destruct (STEP _ _ _ ONE) as (ρ2_src & tid_src & ev_src & ONE' & EV & SS2 & Hr).
-  exists ρ2_src, tid_src, ev_src. do 3 (split; [done|]). by apply LE.
+  constructor; first by intros [[]|].
+  intros [[]|] [[]|] [[]|]; simpl; try done; move => -> -> //.
 Qed.
-Hint Resolve _sim_monotone: paco.
 
-(** The actual simulation *)
-Definition sim: SIM_CFG := paco2 _sim bot2.
+Instance sim_val_po : PreOrder sim_val.
+Proof.
+  constructor; first by (intros []; simpl; naive_solver).
+  intros [|vl1|] [|vl2|] [|vl3|]; simpl; try done; [by etrans|..|naive_solver].
+  move => [Eql1 H1] [Eql2 H2]. rewrite Eql1 Eql2. split; [done|].
+  move => i v1 v3 Eq1 Eq3.
+  destruct (lookup_lt_is_Some_2 vl2 i) as [v2 Eq2].
+  { rewrite Eql2. by eapply lookup_lt_Some. }
+  etrans; [by eapply H1|by eapply H2].
+Qed.
+
+Instance sim_val_expr_po : PreOrder sim_val_expr.
+Proof.
+  constructor.
+  - intros ?. rewrite /sim_val_expr. naive_solver.
+  - move => e1 e2 e3 S1 S2 v3 /S2 [v2 [/S1 [v1 [??]] ?]].
+    exists v1. split; [done|by etrans].
+Qed.
 
 (** Thread simulation *)
+(* This is a simulation between two expressions without any interference.
+  It corresponds to a sequential simulation. *)
+
 Notation SIM_EXPR := (relation expr)%type.
 Notation SIM_THREAD := (SIM_EXPR → expr → state → expr → state → Prop)%type.
 
+(* Generator for the actual simulation *)
 (* TODO: sim_state is not right *)
+(* Target is simulated by source.
+  Adequacy should states that any defined behavior by target is also a defined
+  behavior by source. In the proof of optimizations, we pick target to be the
+  optimized version, and source to be the unoptimized one.
+  This simulation is goal-based, ie. it does not have intermediate observation,
+  and the simulation finalizes at the simulation `sim_terminal` between the
+  non-reducible values.
+  The values can contain any observations of the states in between by reading
+  the memory. Thus the simulation maintains the relation `sim_state` between
+  the states. *)
 Definition _sim_thread (sim_thread: SIM_THREAD) (sim_terminal: SIM_EXPR)
-  (e1_src: expr) (σ0_src: state) (e1_tgt: expr) (σ0_tgt: state) : Prop :=
+  (e1_src: expr) (σ1_src: state) (e1_tgt: expr) (σ1_tgt: state) : Prop :=
   (* Wf ρ1_src → Wf ρ1_tgt → *)
-  ∀ σ1_src σ1_tgt,
-  (* σ1_src, σ1_tgt are new states by other threads' interferences *)
   Wf σ1_src → Wf σ1_tgt →
-  future_state σ0_src σ1_src → future_state σ0_tgt σ1_tgt →
   (* σ1_src, σ1_tgt are related *)
   sim_state σ1_src σ1_tgt →
   (* (1) If `e1_tgt` is terminal, then `e1_src` terminates with τ steps *)
   (terminal e1_tgt → ∃ e2_src σ2_src,
-    rtc thread_τstep (e1_src, σ1_src) (e2_src, σ2_src) ∧
+    rtc thread_step (e1_src, σ1_src) (e2_src, σ2_src) ∧
     sim_state σ2_src σ1_tgt ∧
     terminal e2_src ∧ sim_terminal e2_src e1_tgt) ∧
-  (* (2) If `(e1_tgt, σ1_tgt)` steps to `(e2_tgt, σ2_tgt)` with observation o,
+  (* (2) If `(e1_tgt, σ1_tgt)` steps to `(e2_tgt, σ2_tgt)` with 1+ step,
          then exists `(e2_src, σ2_src)`
-         s.t. `(e1_src, σ1_src)` steps to `(e2_src, σ2_src)` with observation o *)
-  (∀ e2_tgt σ2_tgt ev_tgt efs,
-    thread_step (e1_tgt, σ1_tgt) ev_tgt (e2_tgt, σ2_tgt) efs → ∃ e2_src σ2_src ev_src,
-      thread_1step (e1_src, σ1_src) ev_src (e2_src, σ2_src) ∧
-      externally_equiv ev_src ev_tgt ∧
+         s.t. `(e1_src, σ1_src)` steps to `(e2_src, σ2_src)` with * step
+         and still maintains the relation. *)
+  (∀ e2_tgt σ2_tgt, thread_step (e1_tgt, σ1_tgt) (e2_tgt, σ2_tgt) →
+      ∃ e2_src σ2_src,
+      rtc thread_step (e1_src, σ1_src) (e2_src, σ2_src) ∧
       sim_state σ2_src σ2_tgt ∧
       sim_thread sim_terminal e2_src σ2_src e2_tgt σ2_tgt).
 
-Lemma _sim_thread_monotone : monotone5 _sim_thread.
+Lemma _sim_thread_mono : monotone5 _sim_thread.
 Proof.
-  intros re ???? r r' TS LE σ1_src σ1_tgt WF1 WF2 FT1 FT2 SS.
-  destruct (TS _ _ WF1 WF2 FT1 FT2 SS) as [TERM STEP]. split; [done|].
-  intros e2_tgt σ2_tgt ev_tgt efs ONE.
-  destruct (STEP _ _ _ _ ONE) as (e2_src & σ2_src & ev_src & ONE_src & EV & SS' & Hr).
-  exists e2_src, σ2_src, ev_src. do 3 (split; [done|]). by apply LE.
+  intros re ???? r r' TS LE WF1 WF2 SS.
+  destruct (TS WF1 WF2 SS) as [TERM STEP]. split; [done|].
+  intros e2_tgt σ2_tgt ONE.
+  destruct (STEP _ _ ONE) as (e2_src & σ2_src & STEP1 & SS' & Hr).
+  exists e2_src, σ2_src. do 2 (split; [done|]). by apply LE.
 Qed.
-Hint Resolve _sim_thread_monotone: paco.
+Hint Resolve _sim_thread_mono: paco.
 
+(* Actual simulation *)
 Definition sim_thread: SIM_THREAD := paco5 _sim_thread bot5.
 
-(* Inductive ctx (sim_thread : SIM_THREAD) : SIM_THREAD :=
+Lemma thread_step_wf eσ1 eσ2 :
+  thread_step eσ1 eσ2 → Wf eσ1.2 → Wf eσ2.2.
+Proof. inversion 1. inversion PRIM. by eapply head_step_wf. Qed.
+Lemma rtc_thread_step_wf eσ1 eσ2 :
+  rtc thread_step eσ1 eσ2 → Wf eσ1.2 → Wf eσ2.2.
+Proof.
+  intros SS. induction SS; [done|]. intros WF1. apply IHSS. revert WF1.
+  by apply thread_step_wf.
+Qed.
+
+Definition sim_expr (sim_thread: SIM_THREAD) (sim_terminal : SIM_EXPR)
+  (e_src e_tgt: expr) : Prop :=
+  ∀ σ_src σ_tgt, sim_thread sim_terminal e_src σ_src e_tgt σ_tgt.
+
+Lemma sim_expr_mono st1 st2 : st1 <5= st2 → sim_expr st1 <3= sim_expr st2.
+Proof. intros ST ??? PR ??. by apply ST, PR. Qed.
+
+Inductive ctx (sim_thread : SIM_THREAD) : SIM_THREAD :=
 | CtxIncl (sim_terminal : SIM_EXPR) e_src e_tgt σ_src σ_tgt
     (SIM: sim_thread sim_terminal e_src σ_src e_tgt σ_tgt):
     ctx sim_thread sim_terminal e_src σ_src e_tgt σ_tgt
 | CtxBinOp (sim_terminal : SIM_EXPR)
-    e1_src e1_tgt σ1_src σ1_tgt e2_src e2_tgt σ2_src σ2_tgt
-    (SIM1: sim_thread sim_terminal e1_src σ1_src e1_tgt σ1_tgt)
-    (SIM2: sim_thread sim_terminal e2_src σ1_src e1_tgt σ1_tgt) :
-    ctx sim_thread sim_terminal e1 σ1 e2 σ2. *)
+    op e1_src e1_tgt σ_src σ_tgt e2_src e2_tgt
+    (SIM1: sim_thread sim_terminal e1_src σ_src e1_tgt σ_tgt)
+    (SIM2: sim_expr sim_thread sim_terminal e2_src e2_tgt) :
+    ctx sim_thread sim_terminal (BinOp op e1_src e2_src) σ_src
+                                (BinOp op e1_tgt e2_tgt) σ_tgt
+| CtxApp (sim_terminal : SIM_EXPR)
+    e_src e_tgt σ_src σ_tgt el_src el_tgt
+    (SIMF: sim_thread sim_terminal e_src σ_src e_tgt σ_tgt)
+    (EQL: length el_src = length el_tgt)
+    (SIML: ∀ i ei_tgt, el_tgt !! i = Some ei_tgt →
+      ∃ ei_src, el_src !! i = Some ei_src ∧ 
+      sim_expr sim_thread sim_terminal ei_src ei_tgt) :
+    ctx sim_thread sim_terminal (App e_src el_src) σ_src
+                                (App e_tgt el_tgt) σ_tgt
+| CtxProj (sim_terminal : SIM_EXPR)
+    e1_src e1_tgt σ_src σ_tgt e2_src e2_tgt
+    (SIM1: sim_thread sim_terminal e1_src σ_src e1_tgt σ_tgt)
+    (SIM2: sim_expr sim_thread sim_terminal e2_src e2_tgt) :
+    ctx sim_thread sim_terminal (Proj e1_src e2_src) σ_src
+                                (Proj e1_tgt e2_tgt) σ_tgt
+| CtxConc (sim_terminal : SIM_EXPR)
+    e1_src e1_tgt σ_src σ_tgt e2_src e2_tgt
+    (SIM1: sim_thread sim_terminal e1_src σ_src e1_tgt σ_tgt)
+    (SIM2: sim_expr sim_thread sim_terminal e2_src e2_tgt) :
+    ctx sim_thread sim_terminal (Conc e1_src e2_src) σ_src
+                                (Conc e1_tgt e2_tgt) σ_tgt
+| CtxCopy (sim_terminal : SIM_EXPR)
+    e_src e_tgt σ_src σ_tgt
+    (SIM: sim_thread sim_terminal e_src σ_src e_tgt σ_tgt) :
+    ctx sim_thread sim_terminal (Copy e_src) σ_src
+                                (Copy e_tgt) σ_tgt
+| CtxWrite (sim_terminal : SIM_EXPR)
+    e1_src e1_tgt σ_src σ_tgt e2_src e2_tgt
+    (SIM1: sim_thread sim_terminal e1_src σ_src e1_tgt σ_tgt)
+    (SIM2: sim_expr sim_thread sim_terminal e2_src e2_tgt) :
+    ctx sim_thread sim_terminal (Write e1_src e2_src) σ_src
+                                (Write e1_tgt e2_tgt) σ_tgt
+| CtxDeref (sim_terminal : SIM_EXPR) T
+    e_src e_tgt σ_src σ_tgt
+    (SIM: sim_thread sim_terminal e_src σ_src e_tgt σ_tgt) :
+    ctx sim_thread sim_terminal (Deref e_src T) σ_src
+                                (Deref e_tgt T) σ_tgt
+| CtxRef (sim_terminal : SIM_EXPR)
+    e_src e_tgt σ_src σ_tgt
+    (SIM: sim_thread sim_terminal e_src σ_src e_tgt σ_tgt) :
+    ctx sim_thread sim_terminal (Ref e_src) σ_src
+                                (Ref e_tgt) σ_tgt
+| CtxField (sim_terminal : SIM_EXPR) path
+    e_src e_tgt σ_src σ_tgt
+    (SIM: sim_thread sim_terminal e_src σ_src e_tgt σ_tgt) :
+    ctx sim_thread sim_terminal (Field e_src path) σ_src
+                                (Field e_tgt path) σ_tgt
+| CtxEndCall (sim_terminal : SIM_EXPR)
+    e_src e_tgt σ_src σ_tgt
+    (SIM: sim_thread sim_terminal e_src σ_src e_tgt σ_tgt) :
+    ctx sim_thread sim_terminal (EndCall e_src) σ_src
+                                (EndCall e_tgt) σ_tgt
+| CtxRetag (sim_terminal : SIM_EXPR) kind
+    e1_src e1_tgt σ_src σ_tgt e2_src e2_tgt
+    (SIM1: sim_thread sim_terminal e1_src σ_src e1_tgt σ_tgt)
+    (SIM2: sim_expr sim_thread sim_terminal e2_src e2_tgt) :
+    ctx sim_thread sim_terminal (Retag e1_src kind e2_src) σ_src
+                                (Retag e1_tgt kind e2_tgt) σ_tgt
+| CtxCase (sim_terminal : SIM_EXPR)
+    e_src e_tgt σ_src σ_tgt el_src el_tgt
+    (SIMF: sim_thread sim_terminal e_src σ_src e_tgt σ_tgt)
+    (EQL: length el_src = length el_tgt)
+    (SIML: ∀ i ei_tgt, el_tgt !! i = Some ei_tgt →
+      ∃ ei_src, el_src !! i = Some ei_src ∧
+      sim_expr sim_thread sim_terminal ei_src ei_tgt) :
+    ctx sim_thread sim_terminal (Case e_src el_src) σ_src
+                                (Case e_tgt el_tgt) σ_tgt
+.
 
-(** Composition : composing disjoint configuration preserves
-  configuration simulation *)
+Lemma ctx_mono: monotone5 ctx.
+Proof.
+  intros se e1 σ1 e2 σ2 r r' CTX TS. inversion CTX; subst.
+  - econstructor 1; auto.
+  - econstructor 2; auto. by eapply sim_expr_mono.
+  - econstructor 3; auto. naive_solver eauto using sim_expr_mono.
+  - econstructor 4; auto. by eapply sim_expr_mono.
+  - econstructor 5; auto. by eapply sim_expr_mono.
+  - econstructor 6; auto.
+  - econstructor 7; auto. by eapply sim_expr_mono.
+  - econstructor 8; auto.
+  - econstructor 9; auto.
+  - econstructor 10; auto.
+  - econstructor 11; auto.
+  - econstructor 12; auto. by eapply sim_expr_mono.
+  - econstructor 13; auto. naive_solver eauto using sim_expr_mono.
+Qed.
 
-(** Compatibility: language constructs preserve thread/configuration simulation *)
+(** Compatibility: language constructs preserve thread simulation *)
 
-(** Adequacy: thread simulation implies configuration simulation *)
+Lemma ctx_weak_respectful: weak_respectful5 _sim_thread ctx.
+Proof.
+  econstructor; [by apply ctx_mono|].
+  intros l r M1 M2 se e1 σ1 e2 σ2 CTX. destruct CTX.
+  - (* incl *)
+    eapply _sim_thread_mono; eauto. apply rclo5_incl.
+  - intros WF1 WF2 SS. split.
+    + intros TERM. exfalso. move : TERM. clear. cbv. naive_solver.
+    + destruct (M2 _ _ _ _ _ SIM1 WF1 WF2 SS) as [TT ST].
+      intros e2 σ2. admit.
+  - intros WF1 WF2 SS. split.
+    + intros TERM. exfalso. move : TERM. clear. cbv. naive_solver.
+    + admit.
+  - intros WF1 WF2 SS. split.
+    + intros TERM. exfalso. move : TERM. clear. cbv. naive_solver.
+Abort.
 
-(** Adequacy: congfiguration simulation implies behavior inclusion *)
+Lemma ctx_respectful: respectful5 _sim_thread ctx.
+Proof.
+  econstructor; [by apply ctx_mono|].
+  intros l r M1 M2 se e1 σ1 e2 σ2 CTX. destruct CTX.
+  - eapply _sim_thread_mono; eauto. intros. by econstructor 1.
+  - intros WF1 WF2 SS.
+    destruct (M2 _ _ _ _ _ SIM1 WF1 WF2 SS) as [TT ST]. split.
+    + intros TERM. exfalso. move : TERM. clear. cbv. naive_solver.
+    + intros e_tgt' σ_tgt' STEP.
+Abort.
