theories/tactics.v
@@ -33,8 +33,9 @@ Inductive expr :=
 | EndCall (e : expr)
 | Retag (e : expr) (kind : retag_kind) (call: expr)
 | Case (e : expr) (el : list expr)
-| Fork (e : expr)
-| SysCall (id: nat).
+(* | Fork (e : expr)
+| SysCall (id: nat) *)
+.
 
 Fixpoint to_expr (e : expr) : bor_lang.expr :=
   match e with
@@ -63,8 +64,8 @@ Fixpoint to_expr (e : expr) : bor_lang.expr :=
   | EndCall e => bor_lang.EndCall (to_expr e)
   | Retag e kind call => bor_lang.Retag (to_expr e) kind (to_expr call)
   | Case e el => bor_lang.Case (to_expr e) (map to_expr el)
-  | Fork e => bor_lang.Fork (to_expr e)
-  | SysCall id => bor_lang.SysCall id
+  (* | Fork e => bor_lang.Fork (to_expr e)
+  | SysCall id => bor_lang.SysCall id *)
   end.
 
 Ltac of_expr e :=
@@ -102,8 +103,8 @@ Ltac of_expr e :=
       let e := of_expr e in let call := of_expr call in constr:(Retag e kind call)
   | bor_lang.Case ?e ?el =>
      let e := of_expr e in let el := of_expr el in constr:(Case e el)
-  | bor_lang.Fork ?e => let e := of_expr e in constr:(Fork e)
-  | bor_lang.SysCall ?id => constr:(SysCall e)
+  (* | bor_lang.Fork ?e => let e := of_expr e in constr:(Fork e)
+  | bor_lang.SysCall ?id => constr:(SysCall e) *)
   | @nil bor_lang.expr => constr:(@nil expr)
   | @cons bor_lang.expr ?e ?el =>
       let e := of_expr e in let el := of_expr el in constr:(e::el)
@@ -117,7 +118,7 @@ Ltac of_expr e :=
 
 Fixpoint is_closed (X : list string) (e : expr) : bool :=
   match e with
-  | Val _ _ _ | ClosedExpr _ | SysCall _ => true
+  | Val _ _ _ | ClosedExpr _ (* | SysCall _ *) => true
   | Lit _ | Place _ _ _ | Alloc _ | NewCall => true
   | Var x => bool_decide (x ∈ X)
   | Rec f xl e => is_closed (f :b: xl +b+ X) e
@@ -125,7 +126,7 @@ Fixpoint is_closed (X : list string) (e : expr) : bool :=
       | Proj e1 e2 | Conc e1 e2 => is_closed X e1 && is_closed X e2
   | TVal el => forallb (is_closed X) el
   | App e el | Case e el => is_closed X e && forallb (is_closed X) el
-  | Copy e | AtomRead e| Free e | Fork e | Field e _
+  | Copy e | AtomRead e| Free e (* | Fork e *) | Field e _
     | Deref e _ | Ref e | EndCall e  => is_closed X e
   | CAS e0 e1 e2 => is_closed X e0 && is_closed X e1 && is_closed X e2
   end.
@@ -230,8 +231,8 @@ Fixpoint subst (x : string) (es : expr) (e : expr)  : expr :=
   | EndCall e => EndCall (subst x es e)
   | Retag e kind call => Retag (subst x es e) kind (subst x es call)
   | Case e el => Case (subst x es e) (map (subst x es) el)
-  | Fork e => Fork (subst x es e)
-  | SysCall id => SysCall id
+  (* | Fork e => Fork (subst x es e)
+  | SysCall id => SysCall id *)
   end.
 Lemma to_expr_subst x er e :
   to_expr (subst x er e) = bor_lang.subst x (to_expr er) (to_expr e).
