theories/adequacy.v
@@ -1,0 +1,52 @@
+From stbor Require Import simulation steps_wf.
+From Paco Require Import paco.
+
+Inductive behaviors
+  (step: expr * state → expr * state → Prop)
+  (cfg: expr * state) : val → Prop :=
+| behaviors_term v
+    (TERMINAL: terminal cfg.1)
+    (EQV: sim_val_expr cfg.1 (of_val v)) :
+    behaviors step cfg v
+| behaviors_step cfg' v
+    (STEP: step cfg cfg')
+    (NEXT: behaviors step cfg' v):
+    behaviors step cfg v
+.
+
+(* If c1 ->* c2 -b-> v then c1 -b-> v *)
+Lemma rtc_step_behavior step c1 c2 v
+  (STEPS: rtc step c1 c2) (BEH: behaviors step c2 v):
+  behaviors step c1 v.
+Proof.
+  induction STEPS as [|c1 c2 c3 S1 S2 IH]; [done|]. specialize (IH BEH).
+  econstructor 2; eauto.
+Qed.
+
+Lemma sim_thread_adequacy (cfg_src cfg_tgt: expr * state)
+  (WFS: Wf cfg_src.2) (WFT: Wf cfg_tgt.2)
+  (STATE: sim_state cfg_src.2 cfg_tgt.2)
+  (SIM: sim_thread sim_val_expr cfg_src.1 cfg_src.2 cfg_tgt.1 cfg_tgt.2) :
+  ∀ v, behaviors thread_step cfg_tgt v → behaviors thread_step cfg_src v.
+Proof.
+  intros v BEH. revert cfg_src WFS WFT STATE SIM.
+  induction BEH as [cfg_tgt|cfg_tgt cfg_tgt' v STEP BEH IH];
+    intros cfg_src WFS WFT STATE SIM.
+  - punfold SIM.
+    destruct (SIM WFS WFT STATE) as [TERM ?].
+    destruct (TERM TERMINAL) as (e2 & σ2 & TS & STATE' & TERM' & VAL).
+    eapply (rtc_step_behavior _ _ (e2, σ2)).
+    + by destruct cfg_src.
+    + constructor; [done|simpl]. etrans; eauto.
+  - punfold SIM.
+    destruct (SIM WFS WFT STATE) as [? SS].
+    destruct cfg_src as [e σ]. destruct cfg_tgt' as [e' σ'].
+    destruct (SS e' σ') as (e2 & σ2 & TS & STATE' & SS').
+    { clear -STEP. by destruct cfg_tgt. }
+    simpl in TS. eapply rtc_step_behavior; first by apply TS.
+    apply IH; simpl.
+    + by apply (rtc_thread_step_wf _ _ TS).
+    + by apply (thread_step_wf _ _ STEP).
+    + done.
+    + by inversion SS'.
+Qed.
